rpc/props.v
@@ -44,6 +44,46 @@ Implicit Types v : val.
 Implicit Types (ok : Prop) (failed : bool).
 Implicit Types si : sess_info.
 
+Definition clock k N n :=
+  term_own k N (to_frac_agree (1 / 2) n).
+
+Lemma clock_alloc k N E :
+  ↑N ⊆ E →
+  term_token k E ==∗
+  clock k N 0 ∗
+  clock k N 0 ∗
+  term_token k (E ∖ ↑N).
+Proof.
+iIntros "%sub token".
+iMod (term_own_alloc N (to_frac_agree 1 0) with "token")
+  as "[own token]" => //.
+iFrame. rewrite -Qp.half_half frac_agree_op.
+iDestruct "own" as "[??]". by iFrame.
+Qed.
+
+Lemma clock_agree k N n m :
+  clock k N n -∗
+  clock k N m -∗
+  ⌜n = m⌝.
+Proof.
+iIntros "own1 own2".
+iPoseProof (term_own_valid_2 with "own1 own2") as "%valid".
+rewrite frac_agree_op_valid_L in valid.
+by case: valid.
+Qed.
+
+Lemma clock_update p k N n m :
+  clock k N n -∗
+  clock k N m ==∗
+  clock k N p ∗ clock k N p.
+Proof.
+iIntros "own1 own2". rewrite /clock.
+iMod (term_own_update_2 with "own1 own2") as "[own1 own2]".
+{ apply: (frac_agree_update_2 _ _ _ _ p).
+  by rewrite Qp.half_half. }
+by iFrame.
+Qed.
+
 Variable N : namespace.
 
 Definition never_connected kI kR : iProp :=
@@ -58,98 +98,110 @@ iIntros "!> !> contra".
 by iDestruct (term_meta_token with "contra meta") as "[]".
 Qed.
 
-Definition clock kI kR n :=
-  term_own kI (N.@"client".@kR.@"clock") (to_frac_agree (1 / 2) n).
-
-Lemma clock_alloc kI kR E :
-  ↑N.@"client".@kR.@"clock" ⊆ E →
-  term_token kI E ==∗
-  clock kI kR 0 ∗
-  clock kI kR 0 ∗
-  term_token kI (E ∖ ↑N.@"client".@kR.@"clock").
-Proof.
-iIntros "%sub token".
-iMod (term_own_alloc (N.@"client".@kR.@"clock") (to_frac_agree 1 0)
-       with "token") as "[own token]" => //.
-iFrame. rewrite -Qp.half_half frac_agree_op.
-iDestruct "own" as "[??]". by iFrame.
-Qed.
-
-Lemma clock_agree kI kR n m :
-  clock kI kR n -∗
-  clock kI kR m -∗
-  ⌜n = m⌝.
-Proof.
-iIntros "own1 own2".
-iPoseProof (term_own_valid_2 with "own1 own2") as "%valid".
-rewrite frac_agree_op_valid_L in valid.
-by case: valid.
-Qed.
-
-Lemma clock_update p kI kR n m :
-  clock kI kR n -∗
-  clock kI kR m ==∗
-  clock kI kR p ∗ clock kI kR p.
-Proof.
-iIntros "own1 own2".
-rewrite /clock.
-iMod (term_own_update_2 with "own1 own2") as "[own1 own2]".
-{ apply: (frac_agree_update_2 _ _ _ _ p).
-  by rewrite Qp.half_half. }
-by iFrame.
-Qed.
-
 Definition client_clock kI kR n : iProp :=
-  clock kI kR n ∗
-  ((□ ¬ never_connected kI kR) ∨ clock kI kR 0).
+  clock kI (N.@"client".@kR.@"clock".@1) n.
+
+Definition server_clock' kI kR n : iProp :=
+  clock kI (N.@"client".@kR.@"clock".@2) n.
+
+Definition tick kI kR n : iProp :=
+  client_clock kI kR (S n) ∗
+  server_clock' kI kR n ∗
+  (⌜n = 0⌝ ∗ server_clock' kI kR 0 ∨ □ ¬ never_connected kI kR).
+
+Definition tock kI kR n : iProp :=
+  client_clock kI kR n ∗
+  server_clock' kI kR n ∗
+  (⌜n = 0⌝ ∗ server_clock' kI kR 0 ∨ □ ¬ never_connected kI kR).
 
 Definition server_clock kI kR n : iProp :=
   ⌜n = 0⌝ ∗ never_connected kI kR ∨
-  ⌜n ≠ 0⌝ ∗ clock kI kR n.
+  ⌜n ≠ 0⌝ ∗ server_clock' kI kR n ∗ □ ¬ never_connected kI kR.
 
-Lemma clocks_agree kI kR n m :
+Lemma client_clock_tock kI kR n m :
   client_clock kI kR n -∗
-  server_clock kI kR m -∗
+  tock kI kR m -∗
   ⌜n = m⌝.
 Proof.
-iIntros "[cI [#cS1|cS1]] [[-> cS2]|[% cS2]]".
-- by iDestruct ("cS1" with "cS2") as "[]".
-- by iPoseProof (clock_agree with "cI cS2") as "%".
-- by iPoseProof (clock_agree with "cI cS1") as "->".
-- by iPoseProof (clock_agree with "cS1 cS2") as "<-".
+iIntros "c1 (c2 & _)". iApply (clock_agree with "c1 c2").
 Qed.
 
-Lemma clocks_update kI kR n m :
-  client_clock kI kR n -∗
-  server_clock kI kR m ==∗
-  ⌜n = m⌝ ∗
-  client_clock kI kR (S n) ∗
-  server_clock kI kR (S n).
+Lemma client_clock_alloc kI kR E :
+  ↑N.@"client".@kR.@"clock" ⊆ E →
+  term_token kI E ==∗
+  client_clock kI kR 0 ∗ tock kI kR 0 ∗
+  term_token kI (E ∖ ↑N.@"client".@kR.@"clock").
 Proof.
-iIntros "[cI [#cS1|cS1]] [[-> cS2]|[% cS2]]".
-- by iDestruct ("cS1" with "cS2") as "[]".
-- iPoseProof (clock_agree with "cI cS2") as "%".
-  iMod (clock_update (S n) with "cI cS2") as "[cI cS2]".
+iIntros "%sub token".
+iMod (clock_alloc kI ( N:= N.@"client".@kR.@"clock".@1) with "token")
+  as "(? & ? & token)"; first solve_ndisj.
+iFrame.
+iMod (clock_alloc kI ( N:= N.@"client".@kR.@"clock".@2) with "token")
+  as "(c1 & c2 & token)"; first solve_ndisj.
+iModIntro. iFrame.
+iSplitL "c1".
+- iLeft. by iFrame.
+- iApply (term_token_drop with "token"). solve_ndisj.
+Qed.
+
+Lemma server_clock_alloc kI kR E :
+  ↑N.@"server".@kI ⊆ E →
+  term_token kR E ==∗
+  server_clock kI kR 0 ∗ term_token kR (E ∖ ↑N.@"server".@kI).
+Proof.
+iIntros "%sub token".
+rewrite term_token_difference //. iDestruct "token" as "[??]".
+iFrame. iModIntro. iLeft. by iFrame.
+Qed.
+
+Lemma tock_tick kI kR n m :
+  client_clock kI kR n -∗
+  tock kI kR m ==∗
+  ⌜m = n⌝ ∗
+  client_clock kI kR (S n) ∗
+  tick kI kR n.
+Proof.
+iIntros "client1 (client2 & server1 & ?)".
+iPoseProof (clock_agree with "client1 client2") as "<-".
+iFrame.
+iMod (clock_update (S n) with "client1 client2") as "[??]".
+by iFrame.
+Qed.
+
+Lemma tick_tock kI kR n m :
+  server_clock kI kR n -∗
+  tick kI kR m ==∗
+  ⌜m = n⌝ ∗
+  server_clock kI kR (S n) ∗
+  tock kI kR (S n).
+Proof.
+iIntros "server tick".
+iDestruct "server" as "[(-> & never)|(%n0 & s1 & #first1)]";
+iDestruct "tick" as "(c1 & s2 & [(-> & s3)| #first2])".
+- iMod (first_connection with "never") as "#first".
+  iMod (clock_update 1 with "s2 s3") as "[s2 s3]".
   iModIntro. iSplit => //. iFrame.
-  iSplitR; first by eauto.
-  iRight. iFrame. by eauto.
-- iPoseProof (clock_agree with "cI cS1") as "->".
-  iMod (first_connection with "cS2") as "#?".
-  iMod (clock_update 1 with "cI cS1") as "[cI cS1]".
-  iModIntro. iSplit => //. iFrame.
-  iSplitR; first by eauto. by iRight; iFrame.
-- by iPoseProof (clock_agree with "cS1 cS2") as "<-".
+  iSplitL "s2".
+  + iRight. by iSplit; iFrame.
+  + by iRight.
+- by iPoseProof ("first2" with "never") as "[]".
+- iPoseProof (clock_agree with "s1 s2") as "->".
+  iModIntro. by iSplit => //.
+- iPoseProof (clock_agree with "s1 s2") as "<-".
+  iMod (clock_update (S n) with "s1 s2") as "[s1 s2]".
+  iModIntro. iFrame. iSplit => //.
+  iSplitL; last by eauto.
+  iRight. iFrame. by iSplit.
 Qed.
 
 Definition client_disconnected kI kR n : iProp :=
-  Conn.failure kI kR ∨ client_clock kI kR n.
+  Conn.failure kI kR ∨
+  client_clock kI kR n ∗ tock kI kR n.
 
-Definition client_connected kI kR cs n : iProp := ∃ n1 n0,
-  ⌜n = (n0 + n1)%nat⌝ ∗
-  Conn.connected kI kR Init cs n1 n1 ∗
-  term_meta (si_init_share cs) (isoN.@"conn".@"beg") n0 ∗
+Definition client_connected kI kR cs n : iProp :=
+  Conn.connected kI kR Init cs ∗
   release_token (si_init_share cs) ∗
-  (compromised_session Init cs ∨ client_clock kI kR n).
+  (compromised_session Init cs ∨ client_clock kI kR n ∗ tock kI kR n).
 
 Lemma client_connected_ok kI kR cs n :
   client_connected kI kR cs n -∗
@@ -159,7 +211,7 @@ Lemma client_connected_ok kI kR cs n :
   sign_key kR -∗
   ◇ □ ¬ compromised_session Init cs.
 Proof.
-iIntros "(% & % & % & conn & _)".
+iIntros "(conn & _)".
 by iApply (Conn.connected_ok with "conn").
 Qed.
 
@@ -167,17 +219,15 @@ Lemma client_connected_keys kI kR cs n :
   client_connected kI kR cs n -∗
   ⌜kI = si_init cs⌝ ∗ ⌜kR = si_resp cs⌝.
 Proof.
-iIntros "(% & % & % & conn & _)".
+iIntros "(conn & _)".
 by iPoseProof (Conn.connected_keyE with "conn") as "(-> & -> & _)".
 Qed.
 
 Definition server_disconnected kI kR n : iProp :=
   Conn.failure kI kR ∨ server_clock kI kR n.
 
-Definition server_connected kI kR cs n : iProp := ∃ n1 n0,
-  ⌜n = (n0 + n1)%nat⌝ ∗
-  Conn.connected kI kR Resp cs n1 n1 ∗
-  term_meta (si_resp_share cs) (isoN.@"conn".@"beg") n0 ∗
+Definition server_connected kI kR cs n : iProp :=
+  Conn.connected kI kR Resp cs ∗
   release_token (si_resp_share cs) ∗
   (compromised_session Resp cs ∨ server_clock kI kR n).
 
@@ -189,7 +239,7 @@ Lemma server_connected_ok kI kR cs n :
   sign_key kR -∗
   ◇ □ ¬ compromised_session Resp cs.
 Proof.
-iIntros "(% & % & % & conn & _)".
+iIntros "(conn & _)".
 by iApply (Conn.connected_ok with "conn").
 Qed.
 
@@ -197,7 +247,7 @@ Lemma server_connected_keys kI kR cs n :
   server_connected kI kR cs n -∗
   ⌜kI = si_init cs⌝ ∗ ⌜kR = si_resp cs⌝.
 Proof.
-iIntros "(% & % & % & conn & _)".
+iIntros "(conn & _)".
 by iPoseProof (Conn.connected_keyE with "conn") as "(-> & -> & _)".
 Qed.
 
@@ -210,7 +260,7 @@ Proof.
 iIntros "%sub kI_token".
 rewrite (term_token_difference _ _ _ sub).
 iDestruct "kI_token" as "[kI_token ?]". iFrame.
-iMod (clock_alloc kI (kR := kR)
+iMod (client_clock_alloc kI (kR := kR)
        with "kI_token") as "(c1 & c2 & token)" => //.
 iModIntro. iRight. iFrame.
 Qed.
@@ -227,17 +277,11 @@ iDestruct "token" as "[token ?]". iFrame.
 iModIntro. iRight. iLeft. by eauto.
 Qed.
 
-Definition call_pred φ kI kR si n1 ts : iProp :=
-  ∃ n0,
-    term_meta (si_init_share si) (isoN.@"conn".@"beg") n0 ∗
-    client_clock kI kR (n0 + n1) ∗
-    φ kI kR si (n0 + n1) ts.
+Definition call_pred φ kI kR si ts : iProp :=
+  ∃ n, tick kI kR n ∗ φ kI kR si n ts.
 
-Definition resp_pred φ kI kR si n1 ts : iProp :=
-  ∃ n0,
-    term_meta (si_init_share si) (isoN.@"conn".@"beg") n0 ∗
-    client_clock kI kR (n0 + S n1) ∗
-    φ kI kR si (n0 + n1) ts.
+Definition resp_pred φ kI kR si ts : iProp :=
+  ∃ n, tock kI kR (S n) ∗ φ kI kR si n ts.
 
 Definition rpc_pred (s : string) φ ψ : iProp :=
   seal_pred (N.@s.@"call") (Conn.conn_pred Init (call_pred φ)) ∗
@@ -257,12 +301,12 @@ iModIntro. iApply (seal_pred_token_drop with "token").
 solve_ndisj.
 Qed.
 
-Definition error_pred kI kR si n1 ts : iProp := True.
+Definition error_pred kI kR si ts : iProp := True.
 
-Definition close_pred kI kR si n1 ts : iProp :=
+Definition close_pred kI kR si ts : iProp :=
   released (si_init_share si).
 
-Definition ack_close_pred kI kR si n1 ts : iProp :=
+Definition ack_close_pred kI kR si ts : iProp :=
   False.
 
 Definition ctx : iProp :=
